packages/PCVDMLiftedDescent/PCVDMLiftedDescent.lean
@@ -1,1 +1,0 @@
-import PCVDMLiftedDescent.Basic
